src/HaskStrongToWeak.v
@@ -14,136 +14,234 @@ Require Import HaskLiteralsAndTyCons.
 Require Import HaskWeakTypes.
 Require Import HaskWeakVars.
 Require Import HaskWeak.
+Require Import HaskWeakToCore.
 Require Import HaskStrongTypes.
 Require Import HaskStrong.
-Require Import HaskCoreVars.
 
-Fixpoint mfresh (f:Fresh Kind (fun _ => WeakTypeVar))(lk:list Kind){Γ}(ite:IList _ (fun _ => WeakTypeVar) Γ)
-  : (Fresh Kind (fun _ => WeakTypeVar)) * ((vec WeakTypeVar (length lk)) * (IList _ (fun _ => WeakTypeVar) (app lk Γ))) :=
-  match lk as LK return (Fresh Kind (fun _ => WeakTypeVar)) * ((vec WeakTypeVar (length LK)) *
-                          (IList _ (fun _ => WeakTypeVar) (app LK Γ))) with
-  | nil    => (f,(vec_nil,ite))
-  | k::lk' =>
-    let (f',varsite') := mfresh f lk' ite
-    in  let (vars,ite') := varsite'
-    in  let (v,f'') := next _ _ f' k
-    in (f'',((v:::vars),v::::ite'))
-  end.
+(* Uniques *)
+Variable UniqSupply      : Type.                   Extract Inlined Constant UniqSupply     => "UniqSupply.UniqSupply".
+Variable Unique          : Type.                   Extract Inlined Constant Unique         => "Unique.Unique".
+Variable uniqFromSupply  : UniqSupply -> Unique.   Extract Inlined Constant uniqFromSupply => "UniqSupply.uniqFromSupply".
+Variable splitUniqSupply : UniqSupply -> UniqSupply * UniqSupply.
+    Extract Inlined Constant splitUniqSupply => "UniqSupply.splitUniqSupply".
 
-Fixpoint rawHaskTypeToWeakType (f:Fresh Kind (fun _ => WeakTypeVar)){κ}(rht:RawHaskType (fun _ => WeakTypeVar) κ)
- {struct rht} : WeakType :=
-match rht with
-  | TVar  _  v                 => WTyVarTy v
-  | TCon      tc              => WTyCon tc
-  | TCoerc _ t1 t2 t3          => WCoFunTy (rawHaskTypeToWeakType f t1) (rawHaskTypeToWeakType f t2) (rawHaskTypeToWeakType f t3)
-  | TArrow                    => WFunTyCon
-  | TApp  _ _  t1 t2             => WAppTy (rawHaskTypeToWeakType f t1) (rawHaskTypeToWeakType f t2)
-  | TAll    k rht'            => let (tv,f') := next _ _ f k in WForAllTy tv (rawHaskTypeToWeakType f' (rht' tv))
-  | TCode   t1 t2             => 
-    match (rawHaskTypeToWeakType f t1) with
-      | WTyVarTy ec => WCodeTy ec (rawHaskTypeToWeakType f t2)
-      | impossible  => impossible  (* TODO: find a way to convince Coq this can't happen *)
-    end
-  | TyFunApp    tfc tls         => WTyFunApp tfc (rawHaskTypeListToWeakType f tls)
-end
-with rawHaskTypeListToWeakType (f:Fresh Kind (fun _ => WeakTypeVar)){κ}(rht:RawHaskTypeList κ) :=
-match rht with
-  | TyFunApp_nil   => nil
-  | TyFunApp_cons  κ kl rht' rhtl' => (rawHaskTypeToWeakType f rht')::(rawHaskTypeListToWeakType f rhtl')
-end.
+Inductive UniqM {T:Type} : Type :=
+ | uniqM    : (UniqSupply -> ???(UniqSupply * T)) -> UniqM.
+ Implicit Arguments UniqM [ ].
 
-Definition typeToWeakType (f:Fresh Kind (fun _ => WeakTypeVar))
-  {Γ}{κ}(τ:HaskType Γ κ)(φ:InstantiatedTypeEnv (fun _ => WeakTypeVar) Γ) : WeakType :=
-  rawHaskTypeToWeakType f (τ _ φ).
+Instance UniqMonad : Monad UniqM :=
+{ returnM := fun T (x:T) => uniqM (fun u => OK (u,x))
+; bindM   := fun a b (x:UniqM a) (f:a->UniqM b) =>
+  uniqM (fun u =>
+    match x with
+      | uniqM fa =>
+        match fa u with
+          | Error s   => Error s
+          | OK (u',va) => match f va with
+                           | uniqM fb => fb u'
+                         end
+        end
+    end)
+}.
 
-(* This can be used to turn HaskStrong's with arbitrary expression variables into HaskStrong's which use WeakExprVar's
- * for their variables; those can subsequently be passed to the following function (strongExprToWeakExpr) *)
-(*
-Definition reindexStrongExpr {VV}{HH}{eqVV:EqDecidable VV}{eqHH:EqDecidable HH}
-  {Γ}{Δ}{ξ}{lev}(exp:@Expr VV eqVV Γ Δ ξ lev) : { ξ' : HH -> LeveledHaskType Γ & @Expr HH eqHH Γ Δ ξ' lev }.
-  Defined.
-  *)
+Definition getU : UniqM Unique :=
+  uniqM (fun us => let (us1,us2) := splitUniqSupply us in OK (us1,(uniqFromSupply us2))).
 
-Definition updateITE {Γ:TypeEnv}{TV:Kind->Type}{κ}(tv:TV κ)(ite:InstantiatedTypeEnv TV Γ) : InstantiatedTypeEnv TV (κ::Γ)
-  := tv::::ite.
+Notation "'bind' x = e ; f" := (@bindM _ _ _ _ e (fun x => f)) (x ident, at level 60, right associativity).
+Notation "'return' x" := (returnM x) (at level 100).
+Notation "'failM'  x" := (uniqM (fun _ => Error x)) (at level 100).
 
-Definition coercionToWeakCoercion Γ Δ κ t1 t2 ftv ite (γ:@HaskCoercion Γ Δ (@mkHaskCoercionKind Γ κ t1 t2)) : WeakCoercion :=
-  WCoUnsafe (@typeToWeakType ftv Γ κ t1 ite) (@typeToWeakType ftv Γ κ t2 ite).
-
-Section strongExprToWeakExpr.
+Section HaskStrongToWeak.
 
   Context (hetmet_brak : WeakExprVar).
   Context (hetmet_esc  : WeakExprVar).
 
-  Fixpoint strongExprToWeakExpr {Γ}{Δ}{ξ}{τ}
-    (ftv:Fresh Kind                (fun _ => WeakTypeVar))
-    (fcv:Fresh (WeakType*WeakType) (fun _ => WeakCoerVar))
-    (fev:Fresh WeakType            (fun _ => WeakExprVar))
-    (exp:@Expr _ CoreVarEqDecidable Γ Δ ξ τ)
-    : InstantiatedTypeEnv (fun _ => WeakTypeVar) Γ -> WeakExpr :=
-  match exp as E in @Expr _ _ G D X L return InstantiatedTypeEnv (fun _ => WeakTypeVar) G -> WeakExpr with
-  | EVar  Γ' _ ξ' ev              => fun ite => WEVar (weakExprVar ev (@typeToWeakType ftv Γ' ★  (unlev (ξ' ev)) ite))
-  | ELit  _ _ _ lit _             => fun ite => WELit lit
-  | EApp  Γ' _ _ _ _ _ e1 e2      => fun ite => WEApp (strongExprToWeakExpr ftv fcv fev e1 ite) (strongExprToWeakExpr ftv fcv fev e2 ite)
-  | ELam  Γ'   _ _ _ t _ cv e     => fun ite => WELam (weakExprVar cv (typeToWeakType ftv t ite)) (strongExprToWeakExpr ftv fcv fev e ite)
-  | ELet  Γ' _ _ t _ _ ev e1 e2   => fun ite => WELet (weakExprVar ev (typeToWeakType ftv t ite)) (strongExprToWeakExpr ftv fcv fev e1 ite) (strongExprToWeakExpr ftv fcv fev e2 ite)
-  | EEsc  Γ' _ _ ec t _ e         => fun ite => WEEsc  hetmet_esc (ec _ ite) (strongExprToWeakExpr ftv fcv fev e ite) (typeToWeakType ftv t ite)
-  | EBrak Γ' _ _ ec t _ e         => fun ite => WEBrak hetmet_brak (ec _ ite) (strongExprToWeakExpr ftv fcv fev e ite) (typeToWeakType ftv t ite)
-  | ENote _ _ _ _ n e             => fun ite => WENote n (strongExprToWeakExpr ftv fcv fev e ite)
-  | ETyApp  Γ Δ κ σ τ ξ l       e => fun ite => WETyApp (strongExprToWeakExpr ftv fcv fev e ite) (typeToWeakType ftv τ ite)
-  | ELetRec _ _ _ _ _ vars elrb e => fun ite => WELetRec (exprLetRec2WeakExprLetRec ftv fcv fev elrb ite)(strongExprToWeakExpr ftv fcv fev e ite)
-  | ECast Γ Δ ξ t1 t2 γ l e      => fun ite => WECast  (strongExprToWeakExpr ftv fcv fev e ite)
-                                                 (coercionToWeakCoercion _ _ _ _ _ ftv ite γ)
-  | ECoApp Γ Δ κ σ₁ σ₂ γ σ ξ l e => fun ite => WECoApp (strongExprToWeakExpr ftv fcv fev e ite)
-                                                 (coercionToWeakCoercion _ _ _ _ _ ftv ite γ)
-  | ECase Γ Δ ξ l tc tbranches atypes e alts => fun ite =>
-    let (ev,fev') := next _ _ fev (typeToWeakType ftv (unlev (caseType tc atypes @@ l)) ite) in
-     WECase
-      ev
-      (strongExprToWeakExpr ftv fcv fev' e ite)
-      (@typeToWeakType ftv Γ _ tbranches ite)
-      tc
-      (ilist_to_list (@ilmap _ _ (fun _ => WeakType) _ (fun _ t => typeToWeakType ftv t ite) atypes))
-      ((fix caseBranches
-        (tree:Tree ??{ scb : StrongCaseBranchWithVVs _ _ tc atypes
-                              & Expr (sac_Γ scb Γ)
-                                     (sac_Δ scb Γ atypes (weakCK'' Δ))
-                                     (update_ξ (weakLT'○ξ) (vec2list (vec_map
-                                       (fun x => ((fst x),(snd x @@ weakL' l))) (scbwv_varstypes scb))))
-                                     (weakLT' (tbranches@@l)) })
-        : Tree ??(WeakAltCon * list WeakTypeVar * list WeakCoerVar * list WeakExprVar * WeakExpr) :=
-        match tree with
-          | T_Leaf None     => []
-          | T_Leaf (Some x) => let (scb,e) := x in
-            let (ftv',evarsite') := mfresh ftv _ ite in
-            let fcv' :=  fcv in
-              let (evars,ite') := evarsite' in
-              [(sac_altcon scb,
-                vec2list evars,
-                nil (*FIXME*),
-                map (fun vt => weakExprVar (fst vt) (typeToWeakType ftv' (snd vt) ite')) (vec2list (scbwv_varstypes scb)),
-                strongExprToWeakExpr ftv' fcv' fev' e ite'
-              )]
-          | T_Branch b1 b2  => (caseBranches b1),,(caseBranches b2)
-        end
-      ) alts)
-  | ETyLam _ _ _ k _ _ e          => fun ite =>
-    let (tv,ftv') := next _ _ ftv k in WETyLam tv (strongExprToWeakExpr ftv' fcv fev e (updateITE tv ite))
-  | ECoLam Γ Δ κ σ σ₁ σ₂ ξ l e => fun ite =>
-    let t1' := typeToWeakType ftv σ₁ ite in 
-    let t2' := typeToWeakType ftv σ₂ ite in
-    let (cv,fcv') := next _ _ fcv (t1',t2') in WECoLam cv (strongExprToWeakExpr ftv fcv' fev e ite)
+  Context (mkWeakTypeVar_ : Unique -> Kind                         -> WeakTypeVar).
+  Context (mkWeakCoerVar_ : Unique -> Kind -> WeakType -> WeakType -> WeakCoerVar).
+  Context (mkWeakExprVar_ : Unique ->         WeakType             -> WeakExprVar).
+
+  Definition mkWeakTypeVar (k:Kind)                 : UniqM WeakTypeVar := bind u = getU ; return mkWeakTypeVar_ u k.
+  Definition mkWeakCoerVar (k:Kind)(t1 t2:WeakType) : UniqM WeakCoerVar := bind u = getU ; return mkWeakCoerVar_ u k t1 t2.
+  Definition mkWeakExprVar (t:WeakType)             : UniqM WeakExprVar := bind u = getU ; return mkWeakExprVar_ u t.
+
+  Fixpoint mfresh (lk:list Kind){Γ}(ite:IList _ (fun _ => WeakTypeVar) Γ)
+    : UniqM (((vec WeakTypeVar (length lk)) * (IList _ (fun _ => WeakTypeVar) (app lk Γ)))) :=
+    match lk as LK return UniqM ((vec WeakTypeVar (length LK)) * (IList _ (fun _ => WeakTypeVar) (app LK Γ))) with
+    | nil    => return (vec_nil,ite)
+    | k::lk' => bind v = mkWeakTypeVar k
+              ; bind vars_ite' = mfresh lk' ite
+              ; return ((v:::(fst vars_ite')),v::::(snd vars_ite'))
+    end.
+
+  Fixpoint rawHaskTypeToWeakType {κ}(rht:RawHaskType (fun _ => WeakTypeVar) κ) {struct rht} : UniqM WeakType :=
+  match rht with
+    | TVar  _  v                => return WTyVarTy v
+    | TCon      tc              => return WTyCon tc
+    | TCoerc _ t1 t2 t3         => bind t1' = rawHaskTypeToWeakType t1
+                                 ; bind t2' = rawHaskTypeToWeakType t2
+                                 ; bind t3' = rawHaskTypeToWeakType t3
+                                 ; return WCoFunTy t1' t2' t3'
+    | TArrow                    => return WFunTyCon
+    | TApp  _ _  t1 t2          => bind t1' = rawHaskTypeToWeakType t1
+                                 ; bind t2' = rawHaskTypeToWeakType t2
+                                 ; return WAppTy t1' t2'
+    | TAll    k rht'            => bind tv = mkWeakTypeVar k
+                                 ; bind t' = rawHaskTypeToWeakType (rht' tv)
+                                 ; return WForAllTy tv t'
+    | TCode   t1 t2             => bind t1' = rawHaskTypeToWeakType t1
+                                 ; bind t2' = rawHaskTypeToWeakType t2
+                                 ; match t1' with
+                                     | WTyVarTy ec => return WCodeTy ec t2'
+                                     | _           => failM  "impossible"
+                                   end
+    | TyFunApp    tfc tls       => bind tls' = rawHaskTypeListToWeakType tls
+                                 ; return WTyFunApp tfc tls'
   end
-  with exprLetRec2WeakExprLetRec {Γ}{Δ}{ξ}{τ}{vars}
-    (ftv:Fresh Kind                (fun _ => WeakTypeVar))
-    (fcv:Fresh (WeakType*WeakType) (fun _ => WeakCoerVar))
-    (fev:Fresh WeakType            (fun _ => WeakExprVar))
-    (elrb:@ELetRecBindings _ CoreVarEqDecidable Γ Δ ξ τ vars)
-    : InstantiatedTypeEnv (fun _ => WeakTypeVar) Γ -> Tree ??(WeakExprVar * WeakExpr) :=
-  match elrb as E in ELetRecBindings G D X L V
-     return InstantiatedTypeEnv (fun _ => WeakTypeVar) G -> Tree ??(WeakExprVar * WeakExpr) with
-  | ELR_nil    _ _ _ _           => fun ite => []
-  | ELR_leaf   _ _ ξ' cv v e    => fun ite => [((weakExprVar v (typeToWeakType ftv (unlev (ξ' v)) ite)),(strongExprToWeakExpr ftv fcv fev e ite))]
-  | ELR_branch _ _ _ _ _ _ b1 b2 => fun ite => (exprLetRec2WeakExprLetRec ftv fcv fev b1 ite),, (exprLetRec2WeakExprLetRec ftv fcv fev b2 ite)
+  with rawHaskTypeListToWeakType {κ}(rht:RawHaskTypeList κ) : UniqM (list WeakType) :=
+  match rht with
+    | TyFunApp_nil                   => return nil
+    | TyFunApp_cons  κ kl rht' rhtl' => bind t  = rawHaskTypeToWeakType rht'
+                                      ; bind tl = rawHaskTypeListToWeakType rhtl'
+                                      ; return t::tl
   end.
-End strongExprToWeakExpr.
+  
+  Definition typeToWeakType {Γ}{κ}(τ:HaskType Γ κ)(φ:InstantiatedTypeEnv (fun _ => WeakTypeVar) Γ) : UniqM WeakType :=
+    rawHaskTypeToWeakType (τ _ φ).
+  
+  Definition updateITE {Γ:TypeEnv}{TV:Kind->Type}{κ}(tv:TV κ)(ite:InstantiatedTypeEnv TV Γ) : InstantiatedTypeEnv TV (κ::Γ)
+    := tv::::ite.
+  
+  Definition coercionToWeakCoercion Γ Δ κ t1 t2 ite (γ:@HaskCoercion Γ Δ (@mkHaskCoercionKind Γ κ t1 t2))
+    : UniqM WeakCoercion
+    := bind t1' = @typeToWeakType Γ κ t1 ite
+     ; bind t2' = @typeToWeakType Γ κ t2 ite
+     ; return WCoUnsafe t1' t2'.
+  
+  Fixpoint seqM {a}(l:list (UniqM a)) : UniqM (list a) :=
+    match l with
+      | nil  => return nil
+      | x::y => bind x' = x
+              ; bind y' = seqM y
+              ; return x'::y'
+    end.
+  
+  Context {VV}{eqVV:EqDecidable VV}{toStringVV:ToString VV}.
+  
+  Definition update_χ (χ:VV->???WeakExprVar)(vv:VV)(ev':WeakExprVar) : VV->???WeakExprVar :=
+    fun vv' =>
+      if eqd_dec vv vv'
+      then OK ev'
+      else χ vv'.
+
+  Fixpoint update_χ' (χ:VV->???WeakExprVar)(varsexprs:list (VV * WeakExprVar)) : VV->???WeakExprVar :=
+    match varsexprs with
+      | nil => χ
+      | (vv,wev)::rest => update_χ (update_χ' χ rest) vv wev
+    end.
+
+  Fixpoint exprToWeakExpr {Γ}{Δ}{ξ}{τ}(χ:VV->???WeakExprVar)(exp:@Expr _ eqVV Γ Δ ξ τ)
+    : InstantiatedTypeEnv (fun _ => WeakTypeVar) Γ
+    -> UniqM WeakExpr :=
+    match exp as E in @Expr _ _ G D X L return InstantiatedTypeEnv (fun _ => WeakTypeVar) G -> UniqM WeakExpr with
+    | EVar  Γ' _ ξ' ev              => fun ite => match χ ev with OK v => return WEVar v | Error s => failM s end
+    | EGlobal Γ' _ ξ' t wev         => fun ite => return WEVar wev
+    | ELam  Γ'   _ _ tv _ _ cv e    => fun ite => bind tv' = typeToWeakType tv ite
+                                                ; bind ev' = mkWeakExprVar tv'
+                                                ; bind e'  = exprToWeakExpr (update_χ χ cv ev') e ite
+                                                ; return WELam ev' e'
+    | ELet  Γ' _ _ t _ _ ev e1 e2   => fun ite => bind tv' = typeToWeakType t ite
+                                                ; bind e1' = exprToWeakExpr χ e1 ite
+                                                ; bind ev' = mkWeakExprVar tv'
+                                                ; bind e2' = exprToWeakExpr (update_χ χ ev ev') e2 ite
+                                                ; return WELet ev' e1' e2'
+    | ELit  _ _ _ lit _             => fun ite => return WELit lit
+    | EApp  Γ' _ _ _ _ _ e1 e2      => fun ite => bind e1' = exprToWeakExpr χ e1 ite
+                                                ; bind e2' = exprToWeakExpr χ e2 ite
+                                                ; return WEApp e1' e2'
+    | EEsc  Γ' _ _ ec t _ e         => fun ite => bind t' = typeToWeakType t ite
+                                                ; bind e' = exprToWeakExpr χ e ite
+                                                ; return WEEsc hetmet_esc (ec _ ite) e' t'
+    | EBrak Γ' _ _ ec t _ e         => fun ite => bind t' = typeToWeakType t ite
+                                                ; bind e' = exprToWeakExpr χ e ite
+                                                ; return WEBrak hetmet_brak (ec _ ite) e' t'
+    | ENote _ _ _ _ n e             => fun ite => bind e' = exprToWeakExpr χ e ite
+                                                ; return WENote n e'
+    | ETyApp  Γ Δ κ σ τ ξ l       e => fun ite => bind t' = typeToWeakType τ ite
+                                                ; bind e' = exprToWeakExpr χ e ite
+                                                ; return WETyApp e' t'
+    | ECoApp Γ Δ κ σ₁ σ₂ γ σ ξ l e  => fun ite => bind e' = exprToWeakExpr χ e ite
+                                                ; bind c' = coercionToWeakCoercion _ _ _ _ _ ite γ
+                                                ; return WECoApp e' c'
+    | ECast Γ Δ ξ t1 t2 γ l e      => fun ite  => bind e' = exprToWeakExpr χ e ite
+                                                ; bind c' = coercionToWeakCoercion _ _ _ _ _ ite γ
+                                                ; return WECast e' c'
+    | ETyLam _ _ _ k _ _ e          => fun ite => bind tv = mkWeakTypeVar k
+                                                ; bind e' = exprToWeakExpr χ e (updateITE tv ite)
+                                                ; return WETyLam tv e'
+    | ECoLam Γ Δ κ σ σ₁ σ₂ ξ l e    => fun ite => bind t1' = typeToWeakType σ₁ ite
+                                                ; bind t2' = typeToWeakType σ₂ ite
+                                                ; bind cv  = mkWeakCoerVar κ t1' t2'
+                                                ; bind e'  = exprToWeakExpr χ e ite
+                                                ; return WECoLam cv e'
+    | ECase Γ Δ ξ l tc tbranches atypes escrut alts => 
+         fun ite => bind tscrut'    = typeToWeakType (caseType tc atypes) ite
+                  ; bind vscrut'    = mkWeakExprVar tscrut'
+                  ; bind tbranches' = @typeToWeakType Γ _ tbranches ite
+                  ; bind escrut'    = exprToWeakExpr χ escrut ite
+                  ; bind branches'  =
+                      ((fix caseBranches (tree:Tree ??{scb : StrongCaseBranchWithVVs VV _ _ _ & Expr _ _ _ _  })
+                            : UniqM (Tree ??(WeakAltCon*list WeakTypeVar*list WeakCoerVar*list WeakExprVar*WeakExpr)) :=
+                            match tree with
+                              | T_Leaf None           => return []
+                              | T_Leaf (Some x)       => let (scb,e) := x in
+                                let varstypes := vec2list (scbwv_varstypes scb) in
+                                      bind evars_ite = mfresh _ ite
+                                    ; bind exprvars  = seqM (map (fun vt:VV * HaskType _ ★
+                                                                        => bind tleaf = typeToWeakType (snd vt) (snd evars_ite)
+                                                                         ; bind v' = mkWeakExprVar tleaf
+                                                                         ; return ((fst vt),v'))
+                                                                varstypes)
+                                    ; let χ' := update_χ' χ exprvars in
+                                      bind e'' = exprToWeakExpr χ' e (snd evars_ite)
+                                    ; return [(sac_altcon scb, vec2list (fst evars_ite), nil, (map (@snd _ _) exprvars), e'')]
+                              | T_Branch b1 b2        => bind b1' = caseBranches b1
+                                                       ; bind b2' = caseBranches b2
+                                                       ; return (b1',,b2')
+                            end) alts)
+                  ; bind tys = seqM (ilist_to_list (@ilmap _ _
+                                  (fun _ => UniqM WeakType) _ (fun _ t => typeToWeakType t ite) atypes))
+                  ; return WECase vscrut' escrut' tbranches' tc tys branches'
+
+    | ELetRec _ _ _ _ _ vars elrb e => fun ite => bind vars' = seqM (map (fun vt:VV * HaskType _ ★
+                                                                        => bind tleaf = typeToWeakType (snd vt) ite
+                                                                         ; bind v' = mkWeakExprVar tleaf
+                                                                         ; return ((fst vt),v'))
+                                                                (leaves vars))
+                                                ; let χ' := update_χ' χ vars' in
+                                                  bind elrb' = exprLetRec2WeakExprLetRec χ' elrb ite
+                                                ; bind e'    = exprToWeakExpr χ' e ite
+                                                ; return WELetRec elrb' e'
+    end
+    with exprLetRec2WeakExprLetRec  {Γ}{Δ}{ξ}{τ}(χ:VV->???WeakExprVar){vars}(elrb:@ELetRecBindings _ eqVV Γ Δ ξ τ vars)
+      : InstantiatedTypeEnv (fun _ => WeakTypeVar) Γ -> UniqM (Tree ??(WeakExprVar * WeakExpr)) :=
+    match elrb as E in ELetRecBindings G D X L V
+       return InstantiatedTypeEnv (fun _ => WeakTypeVar) G -> UniqM (Tree ??(WeakExprVar * WeakExpr)) with
+    | ELR_nil    _ _ _ _           => fun ite => return []
+    | ELR_leaf   _ _ ξ' cv v e     => fun ite => bind t'  = typeToWeakType (unlev (ξ' v)) ite
+                                               ; bind e'  = exprToWeakExpr χ e ite
+                                               ; bind v'  = match χ v with Error s => failM s | OK y => return y end
+                                               ; return [(v',e')]
+    | ELR_branch _ _ _ _ _ _ b1 b2 => fun ite => bind b1' = exprLetRec2WeakExprLetRec χ b1 ite
+                                               ; bind b2' = exprLetRec2WeakExprLetRec χ b2 ite
+                                               ; return b1',,b2'
+  end.
+
+
+  Fixpoint strongExprToWeakExpr (us:UniqSupply){Γ}{Δ}{ξ}{τ}(exp:@Expr _ eqVV Γ Δ ξ τ)
+    (ite:InstantiatedTypeEnv (fun _ => WeakTypeVar) Γ)
+    : ???WeakExpr :=
+    match exprToWeakExpr (fun v => Error ("unbound variable " +++ v)) exp ite with
+      uniqM f => f us >>= fun x => OK (snd x)
+      end.
+
+End HaskStrongToWeak.
